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1 Parameters and notation

Our notation is similar to [1].

g = 9.80665 : gravitational acceleration (m/s2)
m = 0.0165 / 0.0295 : NXT2/RCX wheel weight (kg)
R = 0.0216 / 0.0408 : NXT2/RCX wheel radius (m)
w = 0.022 / 0.015 : NXT2/RCX wheel width (m)
Jw = mR2/2 : wheel inertia moment (kg ·m2)
M = 0.55 : body weight (kg)
W = 0.15 : body width (m)
D = 0.045 : body depth (m)
H = 0.158 : body height (m)
L = H/2 : center of mass distance from the wheel axle (m)
Jψ = 0.00805 : body pitch moment of inertia (kg ·m2)
Jφ = 0.005 : body yaw moment of inertia (kg ·m2)
ψ0 = −2 : balanced pitch deviation from upright position (deg)
B = 0.18 : DC motor constant (Nm · s/rad)
K = 20 : DC motor constant (Nm/V )
ψ = : body pitch angle (rad)
θl/r = θ ∓Wφ/(2R) : left/right wheel roll angles (rad)
θ = (θl + θr)/2 : axle midpoint roll angle (rad)
φ = R (θr − θl)/W : body yaw angle (rad)
pl/r = [xl/r yl/r R]T : left/right wheel positions (m)
pm = [xm ym R]T : axle midpoint position (m)
pc = [xc yc zc]

T : body center of mass position (m)
vl/r = : left/right DC motor control power (V)

1.1 Robot position

The position of the center of mass and its derivative can be expressed as

pc = pm + L

 sinψ cosφ
sinψ sinφ

cosψ

 , ṗc = ṗm + L

 ψ̇ cosψ cosφ− φ̇ sinψ sinφ

ψ̇ cosψ sinφ+ φ̇ sinψ cosφ

−ψ̇ sinψ

 , (1)

where pm = (pl + pr)/2. Furthermore, if the φ is constant and the wheels are rotating δθl and δθr radians in
δt seconds, then the wheel positions are changing by

δpl = Rδθl

 cosφ
sinφ

0

 , δpr = Rδθr

 cosφ
sinφ

0

 . (2)

As we take δt→ 0, φ becomes constant on this infinitely short δt interval, and so we obtain

ṗl = R θ̇l

 cosφ
sinφ

0

 , ṗr = R θ̇r

 cosφ
sinφ

0

 , ṗm = R θ̇

 cosφ
sinφ

0

 . (3)
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1.2 Pitch equilibrium

This model assumes that the center of mass is of the robot body is just above the axle at the middle when the
robot is in equilibrium. In real it is not quite true, so one can shift the pitch angle by a constant ψ0 and use
ψ − ψ0 in the model.

But notice that moving the body center of mass also changes the body moment of inertias, Jψ and Jφ, so
these quantities should be identified for a fixed ψ0.

2 Motion equations

The system is divided into two subsystems: the driven segway robot and the driving DC motors.

2.1 Segway robot dynamics

The Lagrangian of the system (without the DC motor) is

L = Et + Er − Ep , (4)

where Et is the translational kinetic energy, Er is the rotational kinetic energy and Ep is the potential energy
defined as

Et =
m

2

(
ẋ2l + ẏ2l

)
+
m

2

(
ẋ2r + ẏ2r

)
+
M

2

(
ẋ2c + ẏ2c + ż2c

)
,

Er =
Jw
2
θ̇2l +

Jw
2
θ̇2r +

Jψ
2
ψ̇2 +

Jφ
2
φ̇2 ,

Ep = mgR+mgR+Mgzc .

(5)

Then to find the equations of motion with respect to ψ, φ and θ, we write the Euler-Lagrange equations for the
Fψ, Fφ, Fθ generalized forces (see appendix A) as

Fψ =
d

dt

(
∂L

∂ψ̇

)
− ∂L

∂ψ
=
(
ML2 + Jψ

)
ψ̈ +

(
MLR cosψ

)
θ̈ −ML2φ̇2 sinψ cosψ −MgL sinψ ,

Fθ =
d

dt

(
∂L

∂θ̇

)
− ∂L

∂θ
=

(
MLR

2
cosψ

)
ψ̈ +

(
mR2 + Jw +

MR2

2

)
θ̈ − MLR

2
ψ̇2 sinψ ,

Fφ =
d

dt

(
∂L

∂φ̇

)
− ∂L

∂φ
=

(
mR2 + Jw +

2R2

W 2

(
ML2 sin2 ψ + Jφ

))
φ̈+

2MR2L2

W 2
φ̇ψ̇ sinψ cosψ .

(6)

2.2 DC motor dynamics

A detailed description of a DC motor model can be found in [3]. However, now we will use a simplified model,
which captures only that the torque is damped by the shaft’s rotational velocity and proportional to the applied
power. So

Fθl/r = −B(θ̇l/r − ψ̇) +Kvl/r , (7)

where B (Nm · rad/s) and K (Nm/V ) are DC motor constants. Then we can express the generalized forces as

Fψ = −(Fθl + Fθr ) = 2B(θ̇ − ψ̇)−K(vl + vr) ,

Fθ =
1

2
(Fθl + Fθr ) = −B(θ̇ − ψ̇) +K

vl + vr
2

,

Fφ =
R

W
(Fθr − Fθl) = −Bφ̇+

R

W
(vr − vl) .

(8)

2.3 State space form

By connecting the two subsystems and rearranging the equations, we get(
ML2 + Jψ

)
ψ̈ + (MLR cosψ)θ̈ = ML2φ̇2 sinψ cosψ +MgL sinψ + 2B

(
θ̇ − ψ̇

)
−K

(
vl + vr

)
,

(MLR cosψ)ψ̈ +
(

(2m+M)R2 + 2Jw

)
θ̈ = MLRψ̇2 sinψ − 2B

(
θ̇ − ψ̇

)
+K

(
vl + vr

)
,(

mR2W 2 +W 2Jw + 2R2
(
ML2 sin2 ψ + Jφ

))
φ̈ = −2MR2L2φ̇ψ̇ sinψ cosψ −BW 2φ̇+RWK

(
vr − vl

)
.

(9)
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By introducing the x = [ψ θ φ ψ̇ θ̇ φ̇ xm ym]T state and the v = [vl vr]
T control, we can write (9) into

H(x) ẋ = f̂(x) + Ĝv , (10)

where H : R8 → R8×8, f̂ : R8 → R8, Ĝ ∈ R8×2,

H(x) =


I3×3 03×2 03×1 03×2

02×3 Ĥ(x) 02×1 01×2

01×3 01×2 ĥ(x) 01×2

02×3 02×2 02×1 I2×2

 , f̂(x) =



ψ̇

θ̇

φ̇

f̂4(x)

f̂5(x)

f̂6(x)

R θ̇ cosφ

R θ̇ sinφ


, Ĝ = K



0 0
0 0
0 0
−1 −1
1 1

−RW RW
0 0
0 0


, (11)

with

Ĥ(x) =

[
Ĥ11 Ĥ12(x)

Ĥ12(x) Ĥ22

]
,

Ĥ11 =ML2 + Jψ
Ĥ12(x) =MLR cosψ

Ĥ22 = (2m+M)R2 + 2Jw

,

ĥ(x) = mR2W 2 +W 2Jw + 2R2
(
ML2 sin2 ψ + Jφ

)
,

f̂4(x) = ML2φ̇2 sinψ cosψ +MgL sinψ + 2B
(
θ̇ − ψ̇

)
,

f̂5(x) = MLRψ̇2 sinψ − 2B
(
θ̇ − ψ̇

)
,

f̂6(x) = −2MR2L2φ̇ψ̇ sinψ cosψ −BW 2φ̇ .

(12)

Notice that det Ĥ(x) > 0 for all x because

det Ĥ(x) =
(
ML2 + Jψ

)(
(2m+M)R2 + 2Jw

)
−
(
MLR cosψ

)2
> M2L2R2 −M2L2R2 cos2 ψ = M2L2R2

(
1− cos2 ψ

)
≥ 0 .

(13)

Furthermore, for all x, we have ĥ(x) > 0 and so detH(x) > 0. Hence, ∃H(x)−1 for all x, and the state space
form becomes

ẋ = H(x)−1
(
f̂(x) + Ĝv

)
= H(x)−1f̂(x) +H(x)−1Ĝv = f(x) +G(x)v , (14)

where

f(x) =



ψ̇

θ̇

φ̇
f4(x)
f5(x)
f6(x)

Rθ̇ cosφ

Rθ̇ sinφ


, G(x) =



0 0
0 0
0 0

g4(x) g4(x)
g5(x) g5(x)
−g6(x) g6(x)

0 0
0 0


, (15)

with

f4(x) =
Ĥ22f̂4(x)− Ĥ12(x)f̂5(x)

Ĥ11Ĥ22 − Ĥ12(x)2
, g4(x) =

−K
(
Ĥ22 + Ĥ12(x)

)
Ĥ11Ĥ22 − Ĥ12(x)2

,

f5(x) =
−Ĥ12(x)f̂4(x) + Ĥ11f̂5(x)

Ĥ11Ĥ22 − Ĥ12(x)2
, g5(x) =

K
(
Ĥ12(x) + Ĥ11

)
Ĥ11Ĥ22 − Ĥ12(x)2

,

f6(x) =
f̂6(x)

ĥ(x)
, g6(x) =

KRW

ĥ(x)
.

(16)

3



A Derivation of the Euler-Lagrange equations

Notice that

ẋc cosφ+ ẏc sinφ = ẋm cosφ+ ẏm sinφ+ Lψ̇ cosψ
(

cos2 φ+ sin2 φ
)

= Rθ̇ + Lψ̇ cosψ ,

ẋc sinφ− ẏc cosφ = ẋm sinφ− ẏm cosφ− Lφ̇ sinψ
(

sin2 φ+ cos2 φ
)

= −Lφ̇ sinψ .
(17)

Then

Fψ =
d

dt

(
∂L

∂ψ̇

)
− ∂L

∂ψ

=
d

dt

(
ML

(
ẋc cosψ cosφ+ ẏc cosψ sinφ− żc sinψ

)
+ Jψψ̇

)
+ML

(
ẋc
(
ψ̇ sinψ cosφ+ φ̇ cosψ sinφ

)
+ ẏc

(
ψ̇ sinψ sinφ− φ̇ cosψ cosφ

)
+ żcψ̇ cosψ − g sinψ

)
=

d

dt

(
ML cosψ

(
ẋc cosφ+ ẏc sinφ

)
+ML2ψ̇ sin2 ψ + Jψψ̇

)
+ML

(
ψ̇ sinψ

(
ẋc cosφ+ ẏc sinφ

)
+ φ̇ cosψ

(
ẋc sinφ− ẏc cosφ

)
− L ψ̇2 sinψ cosψ − g sinψ

)
(17)
=

d

dt

(
MLR θ̇ cosψ +ML2 ψ̇ + Jψψ̇

)
+ML

(
R θ̇ ψ̇ sinψ + L ψ̇2 sinψ cosψ − L φ̇2 cosψ sinψ − L ψ̇2 sinψ cosψ − g sinψ

)
= MLR θ̈ cosψ −MLR θ̇ ψ̇ sinψ +

(
ML2 + Jψ

)
ψ̈ +ML

(
R θ̇ ψ̇ sinψ − L φ̇2 sinψ cosψ − g sinψ

)
=
(
ML2 + Jψ

)
ψ̈ +

(
MLR cosψ

)
θ̈ −ML2 φ̇2 sinψ cosψ −MgL sinψ .

(18)

Furthermore, notice that ∂φ/∂θl/r = ∓R/W and

ẋl/r cosφ+ ẏl/r sinφ = R θ̇l/r cos2 φ+R θ̇l/r sin2 φ = R θ̇l/r ,

ẋl/r sinφ− ẏl/r cosφ = R θ̇l/r cosφ sinφ−R θ̇l/r sinφ cosφ = 0 ,

ẋc cosφ+ ẏc sinφ = R θ̇ cos2 φ+ L
(
ψ̇ cosψ cos2 φ− φ̇ sinψ sinφ cosφ

)
+R θ̇ sin2 φ+ L

(
ψ̇ cosψ sin2 φ+ φ̇ sinψ cosφ sinφ

)
= R θ̇ + Lψ̇ cosψ ,

ẋc sinφ− ẏc cosφ = R θ̇ cosφ sinφ+ L
(
ψ̇ cosψ cosφ sinφ− φ̇ sinψ sin2 φ

)
−R θ̇ sinφ cosφ− L

(
ψ̇ cosψ sinφ cosφ+ φ̇ sinψ cos2 φ

)
= −Lφ̇ sinψ .

(19)
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Then the forces of the left/right axle endpoints can be expressed as

Fθl/r =
d

dt

(
∂L

∂θ̇l/r

)
− ∂L

∂θl/r

=
d

dt

(
mR

(
ẋl/r cosφ+ ẏl/r sinφ

)
+
MR

2

[
ẋc

(
cosφ± 2L

W
sinψ sinφ

)
+ ẏc

(
sinφ∓ 2L

W
sinψ cosφ

)]
+ Jwθ̇l/r ∓

R

W
Jφφ̇

)
∓ mR2

W

(
ẋlθ̇l sinφ− ẏlθ̇l cosφ+ ẋr θ̇r sinφ− ẋr θ̇r cosφ

)
∓ MR

W

(
ẋc
[
R θ̇ sinφ+ L

(
ψ̇ cosψ sinφ+ φ̇ sinψ cosφ

)]
+ ẏc

[
−R θ̇ cosφ+ L

(
− ψ̇ cosψ cosφ+ φ̇ sinψ sinφ

)])
(19)
=

d

dt

(
mR2θ̇l +

MR

2

(
R θ̇ + Lψ̇ cosψ

)
∓ MRL2

W
φ̇ sin2 ψ + Jwθ̇l/r ∓

R

W
Jφφ̇

)
∓ 0∓ MR

W

(
Rθ̇ + Lψ̇ cosψ

)(
− Lφ̇ sinψ

)
± MRL

W
φ̇ sinψ

(
R θ̇ + Lψ̇ cosψ

)
= mR2θ̈l/r +

MR

2

(
R θ̈ + Lψ̈ cosψ − Lψ̇2 sinψ

)
∓ MRL2

W

(
φ̈ sin2 ψ + 2φ̇ψ̇ sinψ cosψ

)
+ Jwθ̈l/r ∓

R

W
Jφφ̈

=
(
mR2 + Jw

)
θ̈l/r +

MR2

2
θ̈ +

(
MRL

2
cosψ

)
ψ̈ − MRL

2
ψ̇2 sinψ

∓ R

W

(
ML2 sin2 ψ + Jφ

)
φ̈∓ 2MRL2

W
φ̇ψ̇ sinψ cosψ .

(20)

By using Fθl and Fθr , we can compute the Fθ, Fφ generalized forces as

Fθ = Fθl
∂θ

∂θl
+ Fθr

∂θ

∂θr
=
Fθl + Fθr

2

=

(
mR2 + Jw +

MR2

2

)
θ̈ +

(
MLR

2
cosψ

)
ψ̈ − MLR

2
ψ̇2 sinψ ,

Fφ = Fθl
∂φ

∂θl
+ Fθr

∂φ

∂θr
=

R

W

(
Fθr − Fθr

)
=

(
mR2 + Jw +

2R2

W 2

(
ML2 sin2 ψ + Jφ

))
φ̈+

2MR2L2

W 2
φ̇ψ̇ sinψ cosψ .

(21)
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